@prefix rdf: <http://www.w3.org/1999/02/22-rdf-syntax-ns#> .
@prefix rdfs: <http://www.w3.org/2000/01/rdf-schema#> .
@prefix owl: <http://www.w3.org/2002/07/owl#> .
@prefix skos: <http://www.w3.org/2004/02/skos/core#> .
@prefix xsd: <http://www.w3.org/2001/XMLSchema#> .
@prefix dct: <http://purl.org/dc/terms/> .
@prefix foaf: <http://xmlns.com/foaf/0.1/> .
@prefix schema: <http://schema.org/> .
@prefix voaf: <http://purl.org/vocommons/voaf#> .
@prefix vann: <http://purl.org/vocab/vann/> .
@prefix wdrs: <http://www.w3.org/2007/05/powder-s#> .
@prefix ah: <http://purl.org/megalod/ms/ah> .
@prefix excav: <http://purl.org/megalod/ms/excav> .


# Metadata #

<http://purl.org/megalod/ms/ah> a voaf:metadataVoc, owl:Ontology;
  dct:title "Asset Description Metadata Schema - ArrowHeads' Metadata Scheme"@en;
  rdfs:label "Asset Description Metadata Schema - ArrowHeads' Metadata Scheme"@en;
  dct:abstract "Arrowhead V1.1 is a RDF vocabulary or a metadata scheme used to describe semantic assets, of archaeologicaçl findings of the Paleoticit."@en;
  dct:creator [
        		   schema:affiliation <http://inesctec.pt>;
		           schema:affiliation <http://fe.up.pt>;
		           schema:affiliation <http://https://cham.fcsh.unl.pt>;
		           schema:affiliation <http://https://www.fcsh.unl.pt>;
  ] ,
  [
    rdfs:seeAlso <http://fe.up.pt/> ;  
    foaf:homepage <https://www.up.pt/portal/en/> ;        
    foaf:name "Mariana Curado Malta" ;
    foaf:maker [
    foaf:name "Mariana Curado Malta";
    foaf:homepage <http://fe.up.pt/>;
    ], [
      schema:affiliation [
      foaf:homepage <https://sigarra.up.pt/feup/pt/fest_geral.cursos_list?pv_num_unico=201906680> ;  
      foaf:name "Domingos Santos"
    ] ;
    rdfs:seeAlso <http://fe.up.pt/> ; 
    foaf:homepage <https://www.up.pt/portal/en/> ;       
    foaf:name "Universidade do Porto"
  ]
  ] ;
	dct:description "This is the RDF encoding of the data Model for the description of the Chalcolithic and Early/Middle Bronze Age arrowheads .";
	dct:modified "2025-05-11"^^xsd:date;
	vann:preferredNamespacePrefix "ah";
	vann:preferredNamespaceUri "http://www.purl.org/megaLOD/ms/ah";
	rdfs:comment "This file specifies the set of RDF classes and properties used in the ArroWheads metadata scheme"@en;
	wdrs:describedby <http://purl.org/megalod/ms/ah> .



              #======<>===============================<>=====#
#===========  #------<>-------------------------------<>-----#  ===========#
#===========  #------<>       CLASSES                 <>-----#  ===========#
#===========  #------<>-------------------------------<>-----#	===========#
              #======<>===============================<>=====#
ah:Arrowhead
	a rdfs:Class;
	rdfs:comment "A Arrowhead."@en;
	rdfs:subClassOf excav:Item;
        rdfs:label "ArrowHead"@en;
	rdfs:label "Ponta de Seta"@pt.

ah:Morphology
	a rdfs:Class;
	rdfs:comment "Morphology of the arrowhead."@en;
	rdfs:comment "Morphologia da Ponta de Seta."@pt;
	rdfs:label "Morfologia"@pt.

ah:Chipping
	a rdfs:Class;
	rdfs:comment "Chipping of the arrowhead."@en;
 	rdfs:label "ArrowHead - Chipping"@en;
	rdfs:label "Chipping"@en.



              #======<>===============================<>=====#
#===========  #------<>-------------------------------<>-----#  ===========#
#===========  #------<>          Properties           <>-----#  ===========#
#===========  #------<>-------------------------------<>-----#	===========#
              #======<>===============================<>=====#

#>-----------------------------------------<#
#>           Object Properties             <#
#>-----------------------------------------<#

ah:hasMorphology
	a rdf:Property,	owl:ObjectProperty;
	rdfs:comment "This property points to an instance of the definition of the morphology of the arrowhead."@en;
	rdfs:label "ArrowHead - morphology"@en;
	rdfs:domain ah:Arrowhead;
	rdfs:range ah:Morphology.

ah:hasChipping
  a rdf:Property, owl:ObjectProperty;
  rdfs:comment "This Property points to an instance of the definition of the chipping of the arrowhead."@en;
  rdfs:label "ArrowHead - has chipping"@en;
  rdfs:domain ah:Arrowhead;
  rdfs:range ah:Chipping.



#>-----------------------------------------<#
#>           Data Properties             <#
#>-----------------------------------------<#

ah:bodyLength
	a rdf:Property,	owl:DataProperty;
	rdfs:comment "This property points to an instance that presents the length of the body of the arrowhead."@en;
	rdfs:label "ArrowHead - bodyLength"@en;
        rdfs:domain ah:Arrowhead;
	rdfs:range excav:TypometryValue.

ah:baseLength
	a rdf:Property,	owl:DataProperty;
	rdfs:comment "This property points to an instance that presents the length of the base of the arrowhead."@en;
	rdfs:label "ArrowHead - baseLength"@en;
        rdfs:domain ah:Arrowhead;
	rdfs:range excav:TypometryValue.

ah:shape
	a rdf:Property,	owl:DataProperty;
	rdfs:comment "This property records the shape of the arrowhead. A good practice is to use the controlled vocabulary  AH-Shape."@en;
	rdfs:label "ArrowHead - shape"@en;
        rdfs:domain ah:Arrowhead;
	rdfs:range xsd:anyURI.

ah:variant
  	a rdf:Property,	owl:DataProperty;
  	rdfs:comment "This property records the variant of the arrowhead. A good practice is to use the controlled vocabulary  AH-Variant."@en;
  	rdfs:label "ArrowHead - Variant"@en;
        rdfs:domain ah:Arrowhead;
  	rdfs:range xsd:anyURI.

ah:point
	a rdf:Property,	owl:DataProperty;
	rdfs:comment "Definition of the tip of the arrowhead. Sharp=True;Fractured=False."@en;
	rdfs:comment "Definição da ponta da ponta de seta. Piquant=True;Não Piquant=False."@pt;
	rdfs:label "Arrowhead-point - point. Sharp=True;Fractured=False"@en;
  	rdfs:label "Arrowhead-point - point. Piquant=True;Não Piquant=False"@pt;
	rdfs:domain ah:Morphology;
	rdfs:range xsd:boolean.

ah:body
	a rdf:Property,	owl:DataProperty;
        rdfs:comment "THis property is used to define the simmetry of the body of the arrowhead. Symmetrical=True; Non-symmetrical=False"@en;
	rdfs:comment "Esta propriedade define a simetria da base da ponta de seta. Simétrica=True; Não simétrica=False";
	rdfs:label "Arrowhead-Morphology - body. Symmetrical=True; Non-symmetrical=False. "@en;
	rdfs:label "Arrowhead-Morphology - body. Simétrica=True; Não Simétrica=False. "@pt;
        rdfs:domain ah:Morphology;
	rdfs:range xsd:boolean.

ah:base
	a rdf:Property,	owl:DataProperty;
	rdfs:comment "This properties defines the base of the arrowhead. A good pratice is to use the controlled vocabulary AH-Base."@en;
	rdfs:comment "Esta propriedade é usada para categorizar a base da ponta de seta. Usar o vocabulário controlado AH-Base."@pt;	
	rdfs:label "ArrowHead - Morphology - Base. A good pratice is to use the Controlled Vocabulary AH-Base. "@en;
	rdfs:label "ArrowHead - Morphology - Base. Uma boa prática é usar o vocabulário controlado AH-Base. "@pt;
	rdfs:domain ah:Morphology;
	rdfs:range xsd:anyURI.

  ah:mode
  	a rdf:Property,	owl:DataProperty;
  	rdfs:comment "Type of retouching incidence, defines the angle formed by the retouching line and the chipping surface. A good pratice is to use the Controlled Vocabulary AH-ChippingMode."@en;
        rdfs:comment "Tipo de incidência do retoque, define o ângulo formado pela linha de retoque e a superfície de lascagem. Usar o vocabulário controlado AH-chippingMode."@pt;  	
  	rdfs:label "Arrowhead-Chipping-mode"@en;
        rdfs:domain ah:Chipping;
  	rdfs:range xsd:anyURI.

ah:amplitude
	a rdf:Property,	owl:DataProperty;
	rdfs:comment "Retouching extension, Marginal=True;Deep=False."@en;
        rdfs:comment "Extensão do retoque, Marginal=True;Profundo=False."@pt;
	rdfs:label "Arrowhead-Chipping-amplitude"@en;
        rdfs:domain ah:Chipping;
	rdfs:range xsd:boolean.

ah:direction
	a rdf:Property,	owl:DataProperty;
	rdfs:comment "It results from the position in which the chip or blade is placed to be retouched. A good pratice is to use the Controlled Vocabulary AH-ChippingDirection."@en;
        rdfs:comment "Resulta da posição em que é colocada a lasca ou lamina para ser retocada. Usar o vocabulário controlado AH-ChippingDirection."@pt;
	rdfs:label "Arrowhead-Chipping-direction"@en;
        rdfs:domain ah:Chipping;
	rdfs:range xsd:anyURI.

ah:orientation
  	a rdf:Property,	owl:DataProperty;
  	rdfs:comment "Angle between the original axis of the part and the line formed by the retouching, Lateral=True;Transverse=False."@en;
    	rdfs:comment "Ângulo entre o eixo primitivo da peça e a linha formada pelo retoque, Lateral=True;Transversal=False."@pt;
  	rdfs:label "Arrowhead-Chipping-Orientation"@en;
 	rdfs:domain ah:Chipping;
  	rdfs:range xsd:boolean.

ah:delineation
	a rdf:Property,	owl:DataProperty;
	rdfs:comment "The retouching gives the margins a shape.. A good pratice is to use the Controlled Vocabulary AH-ChippingDelineation."@en;
 	rdfs:comment "Ângulo entre o eixo primitivo da peça e a linha formada pelo retoque. Usar o vocabulário controlado AH-ChippingDelineation."@pt;
	rdfs:label "Arrowhead-Chipping-delineation"@en;
  	rdfs:domain ah:Chipping;
	rdfs:range ah:anyURI.

ah:chippinglocation-Side
	a rdf:Property,	owl:DataProperty;
	rdfs:comment "The retouching can occupy a position to the left or right of the axis of symmetry and, depending on the axis perpendicular to it, the retouching can be distal, medial or proximal. . A good pratice is to use the COntrolled Vocabulary AH-ChippingLocation."@en;
  	rdfs:comment "Ângulo entre o eixo primitivo da peça e a linha formada pelo retoque. Usar o vocabulário controlado AH-ChippingLocation."@pt;
	rdfs:label "Arrowhead-Chipping Location-lateral"@en;
	rdfs:domain ah:Chipping;
	rdfs:range ah:anyURI.

ah:chippinglocation-Transversal
  	a rdf:Property,	owl:DataProperty;
  	rdfs:comment "The retouching can be distal or proximal and, depending on the edge where it is located, it can occupy a left, right or median position. A good pratice is to use the COntrolled Vocabulary AH-ChippingLocation."@en;
	rdfs:comment "O retoque pode ser distal ou próximal e em função do bordo onde se situa, pode ocupar uma posição à esquerda, à direita, ou mediana. Usar o vocabulário controlado AH-ChippingLocation."@pt;
  	rdfs:label "Arrowhead-Chipping Location-Transversal"@en;
	rdfs:domain ah:Chipping;
  	rdfs:range ah:anyURI

ah:chippingShape
	a rdf:Property,	owl:DataProperty;
	rdfs:comment "Line defined by the edge. A good pratice is to use the Controlled Vocabulary AH-ChippingShape."@en;
	rdfs:comment "Linha definida pelo bordo. Usar o vocabulário controlado AH-ChippingShape."@pt;
	rdfs:label "Arrowhead-Chipping-shape"@en;
  	rdfs:domain ah:Chipping;
	rdfs:range ah:anyURI.

#>---------------------------------------------------------<#
#>      THE END END END END END END END END END            <#
#>---------------------------------------------------------<#
