@prefix rdf: <http://www.w3.org/1999/02/22-rdf-syntax-ns#> .
@prefix rdfs: <http://www.w3.org/2000/01/rdf-schema#> .
@prefix owl: <http://www.w3.org/2002/07/owl#> .
@prefix skos: <http://www.w3.org/2004/02/skos/core#> .
@prefix xsd: <http://www.w3.org/2001/XMLSchema#> .
@prefix dct: <http://purl.org/dc/terms/> .
@prefix foaf: <http://xmlns.com/foaf/0.1/> .
@prefix schema: <http://schema.org/> .
@prefix crm:<http://www.cidoc-crm.org/cidoc-crm/> .
@prefix voaf: <http://purl.org/vocommons/voaf#> .
@prefix vann: <http://purl.org/vocab/vann/> .
@prefix wdrs: <http://www.w3.org/2007/05/powder-s#> .
@prefix ah: <http://purl.org/megalod/ms/ah/> .
@prefix excav: <http://purl.org/megalod/ms/excav/> .


# Metadata #

<http://purl.org/megalod/ms/ah/> a voaf:Vocabulary, owl:Ontology;

  voaf:classNumber 1 ;
  voaf:propertyNumber  17 ;
  dct:title "Asset Description Metadata Schema - Axes' Metadata Scheme"@en;
  rdfs:label "Asset Description Metadata Schema - Axes' Metadata Scheme"@en;
  dct:abstract "Axes V1.0 is a RDF vocabulary or a metadata scheme used to describe semantic assets, of archaeologicaçl findings of the Paleoticit."@en;
  dct:creator [
        		   schema:affiliation <http://inesctec.pt>;
		           schema:affiliation <http://fe.up.pt>;
		           schema:affiliation <https://cham.fcsh.unl.pt>;
		           schema:affiliation <https://www.fcsh.unl.pt>;
  ] ;
	dct:description "This is the RDF encoding of the data Model for the description of the Chalcolithic and Early/Middle Bronze Age axes .";
	dct:modified "2025-05-11"^^xsd:date;
	vann:preferredNamespacePrefix "ah";
	vann:preferredNamespaceUri "http://www.purl.org/megaLOD/ms/ah/";
	rdfs:comment "This file specifies the set of RDF classes and properties used in the Axes metadata scheme"@en;
	wdrs:describedby <http://purl.org/megalod/ms/ah> .



              #======<>===============================<>=====#
#===========  #------<>-------------------------------<>-----#  ===========#
#===========  #------<>       CLASSES                 <>-----#  ===========#
#===========  #------<>-------------------------------<>-----#	===========#
              #======<>===============================<>=====#
ah:Axe
	a rdfs:Class;
	rdfs:comment "An Axe."@en;
	rdfs:subClassOf excav:Item;
        rdfs:label "Axe"@en;
	rdfs:label "Machado"@pt ;
	redf:label "Biface"@fr.



              #======<>===============================<>=====#
#===========  #------<>-------------------------------<>-----#  ===========#
#===========  #------<>          Properties           <>-----#  ===========#
#===========  #------<>-------------------------------<>-----#	===========#
              #======<>===============================<>=====#


#>-----------------------------------------<#
#>           Data Properties             <#
#>-----------------------------------------<#

ah:morphology
	a rdf:Property,	owl:DataProperty;
       	rdfs:comment "The morphology of the axe. Use a term of the controlled vocabulary axe-morphology"@en;
	rdfs:label "Axe - morphology"@en;
        rdfs:domain ah:Axe;
	rdfs:range xsd:anyURI .

ah:crossSection
	a rdf:Property,	owl:DataProperty;
	rdfs:comment "The cross section of the axe. Use a term of the controlled vocabulary axe-morphology."@en;
	rdfs:label "Axe - cross section"@en;
        rdfs:domain ah:Axe;
	rdfs:range xsd:anyURI .

ah:longitudinalSection
	a rdf:Property,	owl:DataProperty;
	rdfs:comment "The Longitudinal Section of the axe. Use a term of the controlled vocabulary  axe-longitudinalSection."@en;
	rdfs:label "Axe - Longitudinal Section"@en;
        rdfs:domain ah:Axe;
	rdfs:range xsd:anyURI.

ah:Polishing
  	a rdf:Property,	owl:DataProperty;
  	rdfs:comment "The Polishing of the axe. Use a term of the controlled vocabulary  axe-Polishing."@en;
  	rdfs:label "Axe - Polishing"@en;
        rdfs:domain ah:Axe;
  	rdfs:range xsd:anyURI.

ah:edge
	a rdf:Property,	owl:DataProperty;
	rdfs:comment "the Edge of the axe. Use a term of the controlled vocabulary  axe-edge."@en;
	rdfs:label "Axe-edge."@en;
	rdfs:domain ah:Axe;
	rdfs:range xsd:anyURI.

ah:body
	a rdf:Property,	owl:DataProperty;
        rdfs:comment "THis property is used to define the simmetry of the body of the arrowhead. Symmetrical=True; Non-symmetrical=False"@en;
	rdfs:comment "Esta propriedade define a simetria da base da ponta de seta. Simétrica=True; Não simétrica=False";
	rdfs:label "Arrowhead-Morphology - body. Symmetrical=True; Non-symmetrical=False. "@en;
	rdfs:label "Arrowhead-Morphology - body. Simétrica=True; Não Simétrica=False. "@pt;
        rdfs:domain ah:Morphology;
	rdfs:range xsd:boolean.

ah:base
	a rdf:Property,	owl:DataProperty;
	rdfs:comment "This properties defines the base of the arrowhead. A good pratice is to use the controlled vocabulary AH-Base."@en;
	rdfs:comment "Esta propriedade é usada para categorizar a base da ponta de seta. Usar o vocabulário controlado AH-Base."@pt;	
	rdfs:label "ArrowHead - Morphology - Base. A good pratice is to use the Controlled Vocabulary AH-Base. "@en;
	rdfs:label "ArrowHead - Morphology - Base. Uma boa prática é usar o vocabulário controlado AH-Base. "@pt;
	rdfs:domain ah:Morphology;
	rdfs:range xsd:anyURI.

  


#>---------------------------------------------------------<#
#>      THE END END END END END END END END END            <#
#>---------------------------------------------------------<#
