@prefix rdf: <http://www.w3.org/1999/02/22-rdf-syntax-ns#> .
@prefix rdfs: <http://www.w3.org/2000/01/rdf-schema#> .
@prefix owl: <http://www.w3.org/2002/07/owl#> .
@prefix xsd: <http://www.w3.org/2001/XMLSchema#> .
@prefix dct: <http://purl.org/dc/terms/> .
@prefix schema: <http://schema.org/> .
@prefix voaf: <http://purl.org/vocommons/voaf#> .
@prefix vann: <http://purl.org/vocab/vann/> .
@prefix wdrs: <http://www.w3.org/2007/05/powder-s#> .
@prefix excav: <https://purl.org/megalod/ms/excav/> .
@prefix axe: <https://purl.org/megalod/ms/axe/> .


# Metadata #

<http://purl.org/megalod/ms/ah/> a voaf:Vocabulary, owl:Ontology;

  voaf:classNumber 1 ;
  voaf:propertyNumber 6 ;
  dct:title "Asset Description Metadata Schema - Axes' Metadata Scheme"@en;
  rdfs:label "Asset Description Metadata Schema - Axes' Metadata Scheme"@en;
  dct:abstract "Axes V1.0 is a RDF vocabulary or a metadata scheme used to describe semantic assets, of archaeologicaçl findings of the Paleoticit."@en;
  dct:creator [
        		   schema:affiliation <http://inesctec.pt>;
		           schema:affiliation <http://fe.up.pt>;
		           schema:affiliation <https://cham.fcsh.unl.pt>;
		           schema:affiliation <https://www.fcsh.unl.pt>;
  ] ;
	dct:description "This is the RDF encoding of the data Model for the description of the Chalcolithic and Early/Middle Bronze Age axes .";
	dct:modified "2025-05-11"^^xsd:date;
	vann:preferredNamespacePrefix "ah";
	vann:preferredNamespaceUri "http://www.purl.org/megalod/ms/axe/";
	rdfs:comment "This file specifies the set of RDF classes and properties used in the Axes metadata scheme"@en;
	wdrs:describedby <http://purl.org/megalod/ms/axe/> .



              #======<>===============================<>=====#
#===========  #------<>-------------------------------<>-----#  ===========#
#===========  #------<>       CLASSES                 <>-----#  ===========#
#===========  #------<>-------------------------------<>-----#	===========#
              #======<>===============================<>=====#
ah:Axe
	a rdfs:Class;
	rdfs:comment "An Axe."@en;
	rdfs:subClassOf excav:Item;
        rdfs:label "Axe"@en;
	rdfs:label "Machado"@pt ;
	redf:label "Biface"@fr.



              #======<>===============================<>=====#
#===========  #------<>-------------------------------<>-----#  ===========#
#===========  #------<>          Properties           <>-----#  ===========#
#===========  #------<>-------------------------------<>-----#	===========#
              #======<>===============================<>=====#


#>-----------------------------------------<#
#>           Data Properties             <#
#>-----------------------------------------<#

ah:morphology
	a rdf:Property,	owl:DataProperty;
       	rdfs:comment "The morphology of the axe. Use a term of the controlled vocabulary axe-morphology"@en;
	rdfs:label "The axe - Morphology"@en;
	rdfs:label "O machado - Morfologia"@pt;	
	rdfs:label "Le biface - Morphologie"@fr;
        rdfs:domain ah:Axe;
	rdfs:range xsd:anyURI .

ah:crossSection
	a rdf:Property,	owl:DataProperty;
	rdfs:comment "The cross section of the axe. Use a term of the controlled vocabulary axe-morphology."@en;
	rdfs:label "The axe - Cross Section"@en;
	rdfs:label "O machado - Secção Transversal"@pt;	
	rdfs:label "Le biface - Section transversale"@fr;
        rdfs:domain ah:Axe;
	rdfs:range xsd:anyURI .

ah:longitudinalSection
	a rdf:Property,	owl:DataProperty;
	rdfs:comment "The longitudinal section of the axe. Use a term of the controlled vocabulary  axe-longitudinalSection."@en;
	rdfs:label "The axe - Longitudinal Section"@en;
	rdfs:label "O machado - Secção Longitudinal"@pt;	
	rdfs:label "Le biface - Section longitudinale"@fr;
        rdfs:domain ah:Axe;
	rdfs:range xsd:anyURI.

ah:polishing
  	a rdf:Property,	owl:DataProperty;
  	rdfs:comment "The polishing of the axe. Use a term of the controlled vocabulary  axe-polishing."@en;
  	rdfs:label "The axe - Polishing"@en;
	rdfs:label "O machado - Polimento"@pt;	
	rdfs:label "Le biface - Polissage"@fr;
        rdfs:domain ah:Axe;
  	rdfs:range xsd:anyURI.

ah:edge
	a rdf:Property,	owl:DataProperty;
	rdfs:comment "The edge of the axe. Use a term of the controlled vocabulary  axe-edge."@en;
	rdfs:label "The Axe-edge."@en;
	rdfs:label "O machado - gume"@pt;	
	rdfs:label "Le biface - tranchant"@fr;
	rdfs:domain ah:Axe;
	rdfs:range xsd:anyURI.

ah:butt
	a rdf:Property,	owl:DataProperty;
	rdfs:comment "The butt of the axe. Use a term of the controlled vocabulary  axe-butt."@en;
	rdfs:label "The Axe - butt."@en;
	rdfs:label "O machado - talão"@pt;	
	rdfs:label "Le biface - talon"@fr;
	rdfs:domain ah:Axe;
	rdfs:range xsd:anyURI.

ah:tracesOfUse
	a rdf:Property,	owl:DataProperty;
        rdfs:comment "The traces of use of the axe.  Use a term of the controlled vocabulary  axe-polishing"@en;
	rdfs:label "The traces of use of the axe. "@en;
	rdfs:label "O machado - Vestígios de Reutilização"@pt;	
	rdfs:label "Le biface - Traces de réutilisation"@fr;
        rdfs:domain ah:Axe;
	rdfs:range xsd:anyURI.

ah:tracesOReuUse
	a rdf:Property,	owl:DataProperty;
        rdfs:comment "The traces of Reuse of the axe.  Use a term of the controlled vocabulary  axe-tracesOfReuse"@en;
	rdfs:label "The traces of use of the axe. "@en;
	rdfs:label "O machado - Vestígios de Reutilização"@pt;	
	rdfs:label "Le biface - Traces de réutilisation"@fr;
        rdfs:domain ah:Axe;
	rdfs:range xsd:anyURI.


ah:tracesOfHaftin
	a rdf:Property,	owl:DataProperty;
        rdfs:comment "The traces of Reuse of the axe.  Use a term of the controlled vocabulary  axe-tracesOfReuse"@en;
	rdfs:label "The traces of use of the axe. "@en;
	rdfs:label "O machado - Vestígios de Reutilização"@pt;	
	rdfs:label "Le biface - Traces de réutilisation"@fr;
        rdfs:domain ah:Axe;
	rdfs:range xsd:anyURI.
  


#>---------------------------------------------------------<#
#>      THE END END END END END END END END END            <#
#>---------------------------------------------------------<#
